Mudança nos nomes

QueeingSystems.v
@@ -5,100 +5,7 @@ Set Implicit Arguments.
 Unset Strict Implicit.
 Unset Printing Implicit Defensive.
 
-Inductive states {Q : Type} : Type :=
-  | sink_state
-  | state (q : Q).
-
-Record dfa (Q E : Type) := {
-  delta : Q -> E -> @states Q;
-  initial_state : Q;
-  is_final : Q -> bool
-}.
-
-(* Extended transition function: *)
-
-Fixpoint extended_delta {Q E : Type} (g : dfa Q E) (q : @states Q) (w : list E) : @states Q :=
-  match q with
-  | sink_state => sink_state
-  | state q' => match w with
-                | [] => state q'
-                | e::w' => extended_delta g (g.(delta) q' e) w'
-                end
-  end.
-
-Theorem dist_extended_delta:
-  forall (Q E : Type) (g : dfa Q E) w w' q,
-    extended_delta g q (w ++ w') =
-    extended_delta g (extended_delta g q w) w'.
-Proof.
-  intros.
-  generalize dependent q.
-  generalize dependent w'.
-  induction w.
-  - intros. simpl. destruct q. reflexivity. reflexivity.
-  - intros. simpl. destruct q.
-    + destruct w'. reflexivity. reflexivity.
-    + rewrite IHw. reflexivity.
-Qed.
-
-(* Generated language: *)
-
-Definition in_language {Q E : Type} (g : dfa Q E) (w : list E) : Prop :=
-  ~ extended_delta g (state g.(initial_state)) w = sink_state.
-
-Notation " x ==> g " := (in_language g x) (at level 60). (* ? *)
-
-Theorem prefix_closed:
-  forall (Q E : Type) (g : dfa Q E) w w',
-    (w ++ w') ==> g -> w ==> g.
-Proof.
-  unfold in_language, not.
-  intros.
-  rewrite dist_extended_delta in H. rewrite H0 in H. apply H.
-  destruct w'. reflexivity. reflexivity.
-Qed.
-
-(*
-Example:
-
-Inductive states1 : Type :=
-  | q0 (* initial state *)
-  | q1
-  | q2 (* final state *).
-
-Inductive events1 : Type :=
-  | a
-  | b.
-
-Definition delta1 (q:states1) (e:events1) : @states states1 :=
-  match q, e with
-  | q0, a => state q1
-  | q1, b => state q2
-  | q2, a => state q1
-  | _, _ => sink_state
-  end.
-
-Definition is_final1 (q:states1) : bool :=
-  match q with
-  | q2 => true
-  | _ => false
-  end.
-
-Definition dfa1 :=
-  {| delta := delta1; initial_state := q0; is_final := is_final1 |}.
-
-Check dfa1.
-
-Compute extended_delta dfa1 (state q0) [a;b;a;b;a;b].
-
-Theorem dfa1_test1 : [a;b;a;b;a;b] ==> dfa1.
-Proof.
-  unfold in_language.
-  unfold not.
-  intros.
-  discriminate H.
-Qed.
-*)
+Require Import DFA.
 
 Require Export Arith_base.
 Require Import BinPos BinInt BinNat Pnat Nnat.
@@ -154,7 +61,7 @@ Proof.
     + rewrite IHw. reflexivity.
 Qed.
 
-Lemma sla3: forall (Q E : Type) (g : dfa Q E) (q : Q) (e : E),
+Lemma extended_delta__delta: forall (Q E : Type) (g : dfa Q E) (q : Q) (e : E),
   extended_delta g (state q) [e] = g.(delta) q e.
 Proof.
   intros.
@@ -164,7 +71,7 @@ Proof.
   reflexivity.
 Qed.
 
-Lemma th2:
+Lemma buffer_count_leq_f:
   forall (Q E : Type) (g : dfa Q (@events E)) (f : @states Q->Z),
     (f(state g.(initial_state)) = 0 /\
       forall (q : Q),
@@ -192,7 +99,7 @@ Proof.
       { rewrite dist_extended_delta. remember (extended_delta g (state (initial_state g)) w). destruct s.
         - apply prefix_closed in H0. unfold in_language in H0. unfold not in H0. symmetry in Heqs. apply H0 in Heqs.
           destruct Heqs.
-        - rewrite sla3. assert (f (delta g q add) >= f (state q) + 1).
+        - rewrite extended_delta__delta. assert (f (delta g q add) >= f (state q) + 1).
           { apply H1. }
           omega. }
       omega.
@@ -204,7 +111,7 @@ Proof.
       { rewrite dist_extended_delta. remember (extended_delta g (state (initial_state g)) w). destruct s.
         - apply prefix_closed in H0. unfold in_language in H0. unfold not in H0. symmetry in Heqs. apply H0 in Heqs.
           destruct Heqs.
-        - rewrite sla3. assert (f (delta g q rem) >= f (state q) - 1).
+        - rewrite extended_delta__delta. assert (f (delta g q rem) >= f (state q) - 1).
           { apply H2. }
           omega. }
       omega.
@@ -216,7 +123,7 @@ Proof.
       { rewrite dist_extended_delta. remember (extended_delta g (state (initial_state g)) w). destruct s.
         - apply prefix_closed in H0. unfold in_language in H0. unfold not in H0. symmetry in Heqs. apply H0 in Heqs.
           destruct Heqs.
-        - rewrite sla3. assert (f (delta g q (other e)) >= f (state q)).
+        - rewrite extended_delta__delta. assert (f (delta g q (other e)) >= f (state q)).
           { apply H3. }
           omega. }
       omega.
@@ -242,7 +149,7 @@ Proof.
     apply H.
   - destruct x.
     + assert (forall w, w ==> g -> buffer_count w <= f (extended_delta g (state g.(initial_state)) w)).
-      { apply th2. split.
+      { apply buffer_count_leq_f. split.
           apply H1. 
           intros. split.
           - apply H2.
@@ -263,4 +170,3 @@ Proof.
     + apply prefix_closed in H0. apply IHw in H0.
       rewrite buffer_other. apply H0.
 Qed.
-
