DFA.v
@@ -1,0 +1,102 @@
+Require Import Coq.Lists.List.
+Import ListNotations.
+
+Set Implicit Arguments.
+Unset Strict Implicit.
+Unset Printing Implicit Defensive.
+
+Inductive states {Q : Type} : Type :=
+  | sink_state
+  | state (q : Q).
+
+Record dfa (Q E : Type) := {
+  delta: Q -> E -> @states Q;
+  initial_state: Q;
+  is_final: Q -> bool
+}.
+
+(* Extended transition function: *)
+
+Fixpoint extended_delta {Q E : Type} (g : dfa Q E) (q : @states Q) (w : list E) : @states Q :=
+  match q with
+  | sink_state => sink_state
+  | state q' => match w with
+                | [] => state q'
+                | e::w' => extended_delta g (g.(delta) q' e) w'
+                end
+  end.
+
+Theorem dist_extended_delta:
+  forall (Q E : Type) (g : dfa Q E) w w' q,
+    extended_delta g q (w ++ w') =
+    extended_delta g (extended_delta g q w) w'.
+Proof.
+  intros.
+  generalize dependent q.
+  generalize dependent w'.
+  induction w.
+  - intros. simpl. destruct q. reflexivity. reflexivity.
+  - intros. simpl. destruct q.
+    + destruct w'. reflexivity. reflexivity.
+    + rewrite IHw. reflexivity.
+Qed.
+
+(* Generated language: *)
+
+Definition in_language {Q E : Type} (g : dfa Q E) (w : list E) : Prop :=
+  ~ extended_delta g (state g.(initial_state)) w = sink_state.
+
+Notation " x ==> g " := (in_language g x) (at level 60). (* ? *)
+
+Theorem prefix_closed:
+  forall (Q E : Type) (g : dfa Q E) w w',
+    (w ++ w') ==> g -> w ==> g.
+Proof.
+  unfold in_language, not.
+  intros.
+  rewrite dist_extended_delta in H. rewrite H0 in H. apply H.
+  destruct w'. reflexivity. reflexivity.
+Qed.
+
+(*
+Example:
+
+Inductive states1 : Type :=
+  | q0 (* initial state *)
+  | q1
+  | q2 (* final state *).
+
+Inductive events1 : Type :=
+  | a
+  | b.
+
+Definition delta1 (q:states1) (e:events1) : @states states1 :=
+  match q, e with
+  | q0, a => state q1
+  | q1, b => state q2
+  | q2, a => state q1
+  | _, _ => sink_state
+  end.
+
+Definition is_final1 (q:states1) : bool :=
+  match q with
+  | q2 => true
+  | _ => false
+  end.
+
+Definition dfa1 :=
+  {| delta := delta1; initial_state := q0; is_final := is_final1 |}.
+
+Check dfa1.
+
+Compute extended_delta dfa1 (state q0) [a;b;a;b;a;b].
+
+Theorem dfa1_test1 : [a;b;a;b;a;b] ==> dfa1.
+Proof.
+  unfold in_language.
+  unfold not.
+  intros.
+  discriminate H.
+Qed.
+*)
+
